IsaSAT: add no restart phases correctly

Weidenbach_Book/IsaSAT_Show.thy
@@ -18,12 +18,14 @@ text \<open>We provide a function to print some information about the state.
 definition println_string :: \<open>String.literal \<Rightarrow> unit\<close> where
   \<open>println_string _ = ()\<close>
 
+definition print_c :: \<open>64 word \<Rightarrow> unit\<close> where
+  \<open>print_c _ = ()\<close>
+
+definition print_uint64 :: \<open>64 word \<Rightarrow> unit\<close> where
+  \<open>print_uint64 _ = ()\<close>
 
 
 subsection \<open>Print Information for IsaSAT\<close>
-
-definition isasat_header :: string where
-  \<open>isasat_header = show ''Conflict | Decision | Propagation | Restarts''\<close>
 
 text \<open>Printing the information slows down the solver by a huge factor.\<close>
 definition isasat_banner_content where
@@ -46,7 +48,17 @@ definition isasat_current_information :: \<open>stats \<Rightarrow> _ \<Rightarr
 \<open>isasat_current_information =
    (\<lambda>(propa, confl, decs, frestarts, lrestarts, uset, gcs, lbds) lcount.
      if confl AND 8191 = 8191 \<comment> \<open>\<^term>\<open>8191 = 8192 - 1\<close>, i.e., we print when all first bits are 1.\<close>
-     then zero_some_stats (propa, confl, decs, frestarts, lrestarts, uset, gcs, lbds)
+     then do{
+       let _ = print_c propa;
+         _ = print_uint64 propa;
+         _ = print_uint64 confl;
+         _ = print_uint64 frestarts;
+         _ = print_uint64 lrestarts;
+         _ = print_uint64 uset;
+         _ = print_uint64 gcs;
+         _ = print_uint64 lbds
+       in
+       zero_some_stats (propa, confl, decs, frestarts, lrestarts, uset, gcs, lbds)}
       else (propa, confl, decs, frestarts, lrestarts, uset, gcs, lbds)
     )\<close>
 
@@ -56,6 +68,10 @@ definition print_current_information :: \<open>stats \<Rightarrow> _ \<Rightarro
      if confl AND 8191 = 8191 then (propa, confl, decs, frestarts, lrestarts, uset, gcs, 0)
      else (propa, confl, decs, frestarts, lrestarts, uset, gcs, lbds))\<close>
 
+lemma print_current_information_isasat_current:
+  \<open>print_current_information = isasat_current_information\<close>
+  by (auto simp: isasat_current_information_def print_current_information_def
+    print_c_def print_uint64_def Let_def zero_some_stats_def intro!: ext)
 
 definition isasat_current_status :: \<open>twl_st_wl_heur \<Rightarrow> twl_st_wl_heur nres\<close> where
 \<open>isasat_current_status =
